Ordering of postconditions and initial states consistent with standard STATE

examples/indexed_effects/IMST.fst
@@ -10,53 +10,60 @@ module W = FStar.Monotonic.Witnessed
 
 //s is at universe level 0 because otherwise sub_effect complains about being too universe polymorphic
 
-let st_post (s:Type0) (a:Type) = a -> s -> Type0
-let st_wp   (a:Type)           = s:Type0 -> (preorder s) -> s -> st_post s a -> Type0
+let st_pre   (s:Type0) = s -> GTot Type0
+let st_post' (s:Type0) (a:Type) (pre:Type) = a -> (_:s{pre}) -> GTot Type0
+let st_post  (s:Type0) (a:Type) = st_post_h' s a True
+let st_wp    (a:Type) = s:Type0 -> (preorder s) -> st_post_h s a -> Tot (st_pre_h s)
+
 
 unfold
-let st_return (a:Type) (x:a) (s:Type0) (rel:preorder s) (s0:s) (p:st_post s a) 
-  = forall v. v == x ==> p v s0
+let st_return (a:Type) (x:a) (s:Type0) (rel:preorder s) (post:st_post s a) (s0:s)
+  = forall v. v == x ==> post v s0
 
 unfold
 let st_bind (r:range) (a:Type) (b:Type)
-            (wp1:st_wp a) (wp2: (a -> Tot (st_wp b))) : st_wp b
-  = fun s rel s0 p -> wp1 s rel s0 (fun x s1 -> wp2 x s rel s1 p)
+            (wp1:st_wp a) (wp2: (a -> Tot (st_wp b))) 
+            (s:Type0) (rel:preorder s) (post:st_post s b) (s0:s) 
+  = wp1 s rel (fun x s1 -> wp2 x s rel post s1) s0
 
 unfold
 let st_if_then_else (a:Type) (p:Type) 
-                      (wp_then:st_wp a) (wp_else:st_wp a) (s:Type0) (rel:preorder s) (s0:s) (post:st_post s a)
-  = l_ITE p (wp_then s rel s0 post) (wp_else s rel s0 post)
+                    (wp_then:st_wp a) (wp_else:st_wp a) 
+                    (s:Type0) (rel:preorder s) (post:st_post s a) (s0:s)
+  = l_ITE p (wp_then s rel post s0) (wp_else s rel post s0)
 
 unfold
-let st_ite (a:Type) (wp:st_wp a) (s:Type0) (rel:preorder s) (s0:s) (post:st_post s a) =
-  wp s rel s0 post
+let st_ite (a:Type) (wp:st_wp a) (s:Type0) (rel:preorder s) (post:st_post s a) (s0:s) 
+  = forall (k:st_post s a).
+	      (forall (x:a) (s1:s).{:pattern (guard_free (k x s1))} post x s1 ==> k x s1)
+	      ==> wp s rel k s0
 
 unfold
-let st_stronger (a:Type) (wp1:st_wp a) (wp2:st_wp a) =
-  forall s rel s0 p. wp1 s rel s0 p ==> wp2 s rel s0 p
+let st_stronger (a:Type) (wp1:st_wp a) (wp2:st_wp a) 
+  = forall (s:Type0) (rel:preorder s) (p:st_post s a) (s0:s) . wp1 s rel p s0 ==> wp2 s rel p s0
 
 unfold
-let st_close (a:Type) (b:Type) 
-             (wp:(b -> GTot (st_wp a))) (s:Type0) (rel:preorder s) (s0:s) (p:st_post s a) =
-  forall x. wp x s rel s0 p
+let st_close (a:Type) (b:Type) (wp:(b -> GTot (st_wp a))) 
+             (s:Type0) (rel:preorder s) (p:st_post s a) (s0:s) 
+  = forall x. wp x s rel p s0
 
 unfold
-let st_assert_p (a:Type) (p:Type) 
-                (wp:st_wp a) (s:Type0) (rel:preorder s) (s0:s) (q:st_post s a) =
-  p /\ wp s rel s0 q
+let st_assert_p (a:Type) (p:Type) (wp:st_wp a) 
+                (s:Type0) (rel:preorder s) (q:st_post s a) (s0:s)
+  = p /\ wp s rel q s0
 
 unfold
-let st_assume_p (a:Type) (p:Type) 
-                (wp:st_wp a) (s:Type0) (rel:preorder s) (s0:s) (q:st_post s a) =
-  p ==> wp s rel s0 q
+let st_assume_p (a:Type) (p:Type) (wp:st_wp a) 
+                (s:Type0) (rel:preorder s) (q:st_post s a) (s0:s)
+  = p ==> wp s rel q s0
 
 unfold
-let st_null (a:Type) (s:Type0) (rel:preorder s) (s0:s) (p:st_post s a) =
-  forall x s1. p x s1
+let st_null (a:Type) (s:Type0) (rel:preorder s) (p:st_post s a) (s0:s)
+  = forall x s1. p x s1
 
 unfold
-let st_trivial (a:Type) (wp:st_wp a) =
-  forall s rel s0. wp s rel s0 (fun _ _ -> True)
+let st_trivial (a:Type) (wp:st_wp a) 
+  = forall s rel s0. wp s rel (fun _ _ -> True) s0
 
 new_effect {
   IMST : result:Type -> wp:st_wp result -> Effect
@@ -77,32 +84,57 @@ new_effect {
 
 (* Standard lifting *)
 
-let lift_div_imst (a:Type) (wp:pure_wp a) (s:Type0) (rel:preorder s) (s0:s) (p:st_post s a) = wp (fun x -> p x s0)
+unfold 
+let lift_div_imst (a:Type) (wp:pure_wp a) (s:Type0) 
+                  (rel:preorder s) (post:st_post s a) (s0:s) 
+  = wp (fun x -> post x s0)
 sub_effect DIV ~> IMST = lift_div_imst
 
 
 (* Non-indexed MST WPs and syntactic sugar for writing effect indices *)
 
-let st_wp'   (a:Type) (s:Type0) = s -> st_post s a -> Type0
+let st_wp' (a:Type) (s:Type0) 
+  = st_post s a -> Tot (st_pre s)
 
 unfold
 let (><) (#a:Type) (sr:(s:Type0 & preorder s)) (wp:st_wp' a (dfst sr)) : st_wp a
-  = fun s rel s0 post -> s == dfst sr /\ (forall x y . rel x y <==> dsnd sr x y) /\ wp s0 post
+  = fun s rel post s0 -> s == dfst sr /\ (forall x y . rel x y <==> dsnd sr x y) /\ wp post s0
 
 
 (* Standard, but now state-and-preorder indexed get, put, witness, and recall actions *)
 
-assume val get (#s:Type0) (#rel:preorder s) (_:unit) : IMST s ((|s , rel|) >< (fun s0 p -> p s0 s0))
+assume val get (#s:Type0) (#rel:preorder s) (_:unit) : IMST s ((|s , rel|) >< (fun p s0 -> p s0 s0))
 
-assume val put (#s:Type0) (#rel:preorder s) (s1:s) : IMST unit ((|s , rel|) >< (fun s0 p -> rel s0 s1 /\ p () s1))
+assume val put (#s:Type0) (#rel:preorder s) (s1:s) : IMST unit ((|s , rel|) >< (fun p s0 -> rel s0 s1 /\ p () s1))
 
 let witnessed (#s:Type) (#rel:preorder s) (p:predicate s) :Type0 = W.witnessed rel p
 
 assume val witness (#s:Type) (#rel:preorder s) (q:predicate s) 
-  : IMST unit ((|s , rel|) >< (fun s0 p -> stable q rel /\ q s0 /\ (witnessed #s #rel q ==> p () s0)))
+  : IMST unit ((|s , rel|) >< (fun p s0 -> stable q rel /\ q s0 /\ (witnessed #s #rel q ==> p () s0)))
   
 assume val recall (#s:Type) (#rel:preorder s) (q:predicate s) 
-  : IMST unit ((|s , rel|) >< (fun s0 p -> stable q rel /\ witnessed #s #rel q /\ (q s0 ==> p () s0)))
+  : IMST unit ((|s , rel|) >< (fun p s0 -> stable q rel /\ witnessed #s #rel q /\ (q s0 ==> p () s0)))
 
 
 
+(* Some sample code *)
+
+let nat_rel' : relation nat
+  = fun i j -> i <= j
+
+let nat_rel : preorder nat = nat_rel'
+
+open FStar.Mul
+
+let f () 
+  : IMST nat ((|nat , nat_rel|) >< (fun p s0 -> forall s1 . s1 > s0 ==>  p s0 s1))
+  = let s0 = get #nat #nat_rel () in 
+    put #nat #nat_rel (s0 + 1);
+    let s1 = get #nat #nat_rel () in
+    assert (s1 > 0);
+    witness #nat #nat_rel (fun n -> n > 0);
+    put #nat #nat_rel (s1 * 42);
+    recall #nat #nat_rel (fun n -> n > 0);
+    let s2 = get #nat #nat_rel () in
+    assert (s2 > 0);
+    s0
