examples/indexed_effects/IST.fst
@@ -9,94 +9,116 @@ module IST
 
 //s is at universe level 0 because otherwise sub_effect complains about being too universe polymorphic
 
-let st_post (s:Type0) (a:Type) = a -> s -> Type0
-let st_wp   (a:Type)           = s:Type0 -> s -> st_post s a -> Type0
 
-unfold
-let st_return (a:Type) (x:a) (s:Type0) (s0:s) (p:st_post s a) 
-  = forall v. v == x ==> p v s0
+let st_pre   (s:Type0) = s -> GTot Type0
+let st_post' (s:Type0) (a:Type) (pre:Type) = a -> (_:s{pre}) -> GTot Type0
+let st_post  (s:Type0) (a:Type) = st_post_h' s a True
+let st_wp    (a:Type) = s:Type0 -> st_post_h s a -> Tot (st_pre_h s)
 
-unfold
-let st_bind (r:range) (a:Type) (b:Type)
-            (wp1:st_wp a) (wp2: (a -> Tot (st_wp b))) : st_wp b
-  = fun s s0 p -> wp1 s s0 (fun x s1 -> wp2 x s s1 p)
+unfold 
+let st_return  (a:Type) (x:a) (s:Type0) (post:st_post s a) 
+  = post x
 
-unfold
-let st_if_then_else (a:Type) (p:Type) 
-                      (wp_then:st_wp a) (wp_else:st_wp a) (s:Type0) (s0:s) (post:st_post s a)
-  = l_ITE p (wp_then s s0 post) (wp_else s s0 post)
+unfold 
+let st_bind_wp (r1:range) (a:Type) (b:Type)
+               (wp1:st_wp a) (wp2:(a -> GTot (st_wp b)))
+               (s:Type0) (post:st_post s b) (s0:s) 
+  = wp1 s (fun a s1 -> wp2 a s post s1) s0
 
-unfold
-let st_ite (a:Type) (wp:st_wp a) (s:Type0) (s0:s) (post:st_post s a) =
-  wp s s0 post
+unfold 
+let st_if_then_else (a:Type) (p:Type)
+                    (wp_then:st_wp a) (wp_else:st_wp a)
+                    (s:Type0) (post:st_post_h s a) (s0:s) 
+  = l_ITE p (wp_then s post s0) (wp_else s post s0)
 
-unfold
-let st_stronger (a:Type) (wp1:st_wp a) (wp2:st_wp a) =
-  forall s s0 p. wp1 s s0 p ==> wp2 s s0 p
+unfold 
+let st_ite_wp (a:Type) (wp:st_wp a)
+              (s:Type0) (post:st_post s a) (s0:s) 
+  = forall (k:st_post s a).
+	      (forall (x:a) (s1:s).{:pattern (guard_free (k x s1))} post x s1 ==> k x s1)
+	      ==> wp s k s0
 
-unfold
-let st_close (a:Type) (b:Type) 
-               (wp:(b -> GTot (st_wp a))) (s:Type0) (s0:s) (p:st_post s a) =
-  forall x. wp x s s0 p
+unfold 
+let st_stronger (a:Type) (wp1:st_wp a)
+                (wp2:st_wp a)
+  = forall (s:Type0) (post:st_post s a) (s0:s). wp1 s post s0 ==> wp2 s post s0
 
-unfold
-let st_assert_p (a:Type) (p:Type) 
-                  (wp:st_wp a) (s:Type0) (s0:s) (q:st_post s a) =
-  p /\ wp s s0 q
+unfold 
+let st_close_wp (a:Type) (b:Type)
+                (wp:(b -> GTot (st_wp a)))
+                (s:Type0) (post:st_post s a) (s0:s) 
+  = (forall (x:b). wp x s post s0)
 
-unfold
-let st_assume_p (a:Type) (p:Type) 
-                  (wp:st_wp a) (s:Type0) (s0:s) (q:st_post s a) =
-  p ==> wp s s0 q
+unfold 
+let st_assert_p (a:Type) (p:Type)
+                (wp:st_wp a)
+                (s:Type0)
+                (q:st_post s a) (s0:s) 
+  = p /\ wp s q s0
 
-unfold
-let st_null (a:Type) (s:Type0) (s0:s) (p:st_post s a) =
-  forall x s1. p x s1
+unfold 
+let st_assume_p (a:Type) (p:Type)
+                (wp:st_wp a)
+                (s:Type0)
+                (q:st_post s a) (s0:s) 
+  = p ==> wp s q s0
 
-unfold
-let st_trivial (a:Type) (wp:st_wp a) =
-  forall s s0. wp s s0 (fun _ _ -> True)
+unfold 
+let st_null_wp (a:Type) (s:Type0) 
+               (p:st_post s a) (s0:s) 
+  = forall (x:a) (s0:s). p x s0
+
+unfold 
+let st_trivial (a:Type) (wp:st_wp a) 
+  = forall s s0. wp s (fun r s1 -> True) s0
 
 new_effect {
   STATE : result:Type -> wp:st_wp result -> Effect
   with 
      //repr         = s:Type0 -> s -> M (a * s) //pi-types currently not supported by DM4F
        return_wp    = st_return
-     ; bind_wp      = st_bind
+     ; bind_wp      = st_bind_wp
      ; if_then_else = st_if_then_else
-     ; ite_wp       = st_ite
+     ; ite_wp       = st_ite_wp
      ; stronger     = st_stronger
-     ; close_wp     = st_close
+     ; close_wp     = st_close_wp
      ; assert_p     = st_assert_p
      ; assume_p     = st_assume_p
-     ; null_wp      = st_null
+     ; null_wp      = st_null_wp
      ; trivial      = st_trivial
 }
 
 
 (* Standard lifting *)
 
-let lift_div_st (a:Type) (wp:pure_wp a) (s:Type0) (s0:s) (p:st_post s a) = wp (fun x -> p x s0)
+unfold 
+let lift_div_st (a:Type) (wp:pure_wp a) 
+                (s:Type0) (p:st_post s a) (s0:s) 
+  = wp (fun x -> p x s0)
 sub_effect DIV ~> STATE = lift_div_st
 
 
 (* Non-indexed ST WPs and syntactic sugar for writing effect indices *)
 
-let st_wp'   (a:Type) (s:Type0) = s -> st_post s a -> Type0
+let st_wp'   (a:Type) (s:Type0) = st_post s a -> st_pre s
 
 unfold
 let (><) (#a:Type) (s:Type0) (wp:st_wp' a s) : st_wp a
-  = fun s' s0 post -> s == s' /\ wp s0 post
+  = fun s' post s0 -> s == s' /\ wp post s0
 
 
 (* Standard, but now state-indexed get and put actions *)
 
-assume val get (#s:Type0) (_:unit) : STATE s (s >< (fun s0 p -> p s0 s0))
+assume val get (#s:Type0) (_:unit) : STATE s (s >< (fun p s0 -> p s0 s0))
 
-assume val put (#s:Type0) (s1:s) : STATE unit (s >< (fun s0 p -> p () s1))
+assume val put (#s:Type0) (s1:s) : STATE unit (s >< (fun p s0 -> p () s1))
 
 
 (* Some sample code *)
 
-let f (i:int) : STATE int (int >< (fun s0 p -> p s0 (s0 + i)))
-  = let j = get () in put (i + j) ; j
+let f () : STATE unit (int >< (fun p s0 -> p () s0))
+  = () // without setting unfold for lift_div_st this fails
+
+let g (i:nat{i > 0}) 
+  : STATE int (int >< (fun p s0 -> forall k . k > s0 ==> p s0 k))
+  = let j = get () in put (i + j); j
